feat: add intersection on `ExtDTreeMap`/`ExtTreeMap`/`ExtTreeSet` (#11292)
This PR adds intersection operation on
`ExtDTreeMap`/`ExtTreeMap`/`ExtTreeSet` and proves several lemmas about
it.

src/Std/Data/ExtDTreeMap/Basic.lean
@@ -918,6 +918,17 @@ def union [TransCmp cmp] (m₁ m₂ : ExtDTreeMap α β cmp) : ExtDTreeMap α β
 
 instance [TransCmp cmp] : Union (ExtDTreeMap α β cmp) := ⟨union⟩
 
+@[inline, inherit_doc DTreeMap.union]
+def inter [TransCmp cmp] (m₁ m₂ : ExtDTreeMap α β cmp) : ExtDTreeMap α β cmp := lift₂ (fun x y : DTreeMap α β cmp => mk (x.inter y))
+  (fun a b c d equiv₁ equiv₂ => by
+    simp only [DTreeMap.inter_eq, mk'.injEq]
+    apply Quotient.sound
+    apply DTreeMap.Equiv.inter_congr
+    . exact equiv₁
+    . exact equiv₂) m₁ m₂
+
+instance [TransCmp cmp] : Inter (ExtDTreeMap α β cmp) := ⟨inter⟩
+
 instance [TransCmp cmp] [Repr α] [(a : α) → Repr (β a)] : Repr (ExtDTreeMap α β cmp) where
   reprPrec m prec := Repr.addAppParen ("Std.ExtDTreeMap.ofList " ++ repr m.toList) prec
 
