src/Std/Data/DTreeMap/Raw/Lemmas.lean
@@ -2691,6 +2691,25 @@ theorem not_mem_inter_of_not_mem_right [TransCmp cmp] (h₁ : t₁.WF) (h₂ : t
   simp only [Inter.inter]
   exact Impl.contains_inter!_eq_false_of_contains_eq_false_right h₁ h₂ h
 
+theorem Equiv.inter_left [TransCmp cmp] {t₃ : Raw α β cmp}
+    (h₁ : t₁.WF) (h₂ : t₂.WF) (h₃ : t₃.WF) (equiv : t₁ ~m t₂) :
+    (t₁ ∩ t₃).Equiv (t₂ ∩ t₃) := by
+  simp only [Inter.inter]
+  exact ⟨@Impl.Equiv.inter!_left _ _ ⟨cmp⟩ t₁.inner t₂.inner t₃.inner _ h₁.out h₂.out h₃.out equiv.1⟩
+
+theorem Equiv.inter_right [TransCmp cmp] {t₃ : Raw α β cmp}
+    (h₁ : t₁.WF) (h₂ : t₂.WF) (h₃ : t₃.WF) (equiv : t₂ ~m t₃) :
+    (t₁ ∩ t₂).Equiv (t₁ ∩ t₃) := by
+  simp only [Inter.inter]
+  exact ⟨@Impl.Equiv.inter!_right _ _ ⟨cmp⟩ t₁.inner t₂.inner t₃.inner _ h₁.out h₂.out h₃.out equiv.1⟩
+
+theorem Equiv.inter_congr [TransCmp cmp] {t₃ t₄ : Raw α β cmp}
+    (h₁ : t₁.WF) (h₂ : t₂.WF) (h₃ : t₃.WF) (h₄ : t₄.WF)
+    (equiv₁ : t₁ ~m t₃) (equiv₂ : t₂ ~m t₄) :
+    (t₁ ∩ t₂).Equiv (t₃ ∩ t₄) := by
+  simp only [Inter.inter]
+  exact ⟨@Impl.Equiv.inter!_congr _ _ ⟨cmp⟩ t₁.inner t₂.inner t₃.inner t₄.inner _ h₁.out h₂.out h₃.out h₄.out equiv₁.1 equiv₂.1⟩
+
 /- get? -/
 theorem get?_inter [TransCmp cmp] [LawfulEqCmp cmp] (h₁ : t₁.WF) (h₂ : t₂.WF)
     {k : α} :
