src/Std/Data/TreeSet/Raw/Lemmas.lean
@@ -668,6 +668,22 @@ theorem not_mem_inter_of_not_mem_right [TransCmp cmp]
     k ∉ t₁ ∩ t₂ :=
   TreeMap.Raw.not_mem_inter_of_not_mem_right h₁ h₂ not_mem
 
+theorem Equiv.inter_left [TransCmp cmp] {t₃ : Raw α cmp}
+    (h₁ : t₁.WF) (h₂ : t₂.WF) (h₃ : t₃.WF) (equiv : t₁ ~m t₂) :
+    (t₁ ∩ t₃).Equiv (t₂ ∩ t₃) :=
+  ⟨TreeMap.Raw.Equiv.inter_left h₁ h₂ h₃ equiv.1⟩
+
+theorem Equiv.inter_right [TransCmp cmp] {t₃ : Raw α cmp}
+    (h₁ : t₁.WF) (h₂ : t₂.WF) (h₃ : t₃.WF) (equiv : t₂ ~m t₃) :
+    (t₁ ∩ t₂).Equiv (t₁ ∩ t₃) :=
+  ⟨TreeMap.Raw.Equiv.inter_right h₁ h₂ h₃ equiv.1⟩
+
+theorem Equiv.inter_congr [TransCmp cmp] {t₃ t₄ : Raw α cmp}
+    (h₁ : t₁.WF) (h₂ : t₂.WF) (h₃ : t₃.WF) (h₄ : t₄.WF)
+    (equiv₁ : t₁ ~m t₃) (equiv₂ : t₂ ~m t₄) :
+    (t₁ ∩ t₂).Equiv (t₃ ∩ t₄) :=
+  ⟨TreeMap.Raw.Equiv.inter_congr h₁ h₂ h₃ h₄ equiv₁.1 equiv₂.1⟩
+
 /- get? -/
 theorem get?_inter [TransCmp cmp]
     (h₁ : t₁.WF) (h₂ : t₂.WF)
